intro, laws and theorems

PSBP/Specifications/ProgramSpecifications.lean
@@ -5,12 +5,92 @@ class Functional
 
 export Functional (asProgram)
 
-export Functional (asProgram)
+class Functorial
+    (program : Type → Type → Type) where
+  andThenF {α β γ : Type} :
+    program α β → (β → γ) → program α γ
+
+export Functorial (andThenF)
+
+infixl:50 " >-> " => andThenF
+
+class Sequential
+    (program : Type → Type → Type) where
+  andThen {α β γ : Type} :
+    program α β → program β γ → program α γ
+
+export Sequential (andThen)
+
+infixl:50 " >=> " => andThen
+
+class Creational
+    (program : Type → Type → Type) where
+  product {α β γ : Type} :
+    program α β → program α γ → program α (β × γ)
+
+export Creational (product)
+
+infixl:60 " &&& " => product
+
+class Conditional
+    (program : Type → Type → Type) where
+  sum {α β γ : Type} :
+    program γ α → program β α → program (γ ⊕ β) α
+
+export Conditional (sum)
+
+infixl:55 " ||| " => sum
+
+--
+-- Functional
+--
 
 def identity
     [Functional program] :
   program α α :=
     asProgram id
+
+def first
+    [Functional program] :
+  program (α × β) α :=
+    asProgram λ (α, _) => α
+
+def second
+    [Functional program] :
+  program (α × β) β :=
+    asProgram λ (_, β) => β
+
+def applyAtFirst
+    [Functional program] :
+  (α → β) → program (α × γ) (β × γ) :=
+    λ αfβ => asProgram λ (α, γ) => (αfβ α, γ)
+
+def applyAtSecond
+    [Functional program] :
+  (β → γ) → program (α × β) (α × γ) :=
+    λ βfγ => asProgram λ (α, β) => (α, βfγ β)
+
+def assoc
+    [Functional program] :
+  program ((α × β) × γ) (α × (β × γ)) :=
+    asProgram (λ ((a, b), c) => (a, (b, c)))
+
+def swap
+    [Functional program] :
+  program (α × β) (β × α) :=
+    asProgram  λ (a, β) => (β, a)
+
+def left
+    [Functional program] :
+  program γ (γ ⊕ β) :=
+    asProgram .inl
+
+def right
+    [Functional program] :
+  program β (γ ⊕ β) :=
+    asProgram .inr
+
+-- positional
 
 def positionOne
     [Functional program] :
@@ -27,44 +107,11 @@ def positionOneAndTwo
   program ((σ × β) × α) (α × β) :=
     asProgram λ ((_, β), α) => (α, β)
 
-def first
-    [Functional program] :
-  program (α × β) α :=
-    asProgram λ (α, _) => α
-
-def second
-    [Functional program] :
-  program (α × β) β :=
-    asProgram  λ (_, β) => β
-
 -- ...
 
-class Functorial
-    (program : Type → Type → Type) where
-  andThenF {α β γ : Type} :
-    program α β → (β → γ) → program α γ
-
-export Functorial (andThenF)
-
-infixl:50 " >-> " => andThenF
-
-class Creational
-    (program : Type → Type → Type) where
-  product {α β γ : Type} :
-    program α β → program α γ → program α (β × γ)
-
-export Creational (product)
-
-infixl:60 " &&& " => product
-
-class Sequential
-    (program : Type → Type → Type) where
-  andThen {α β γ : Type} :
-    program α β → program β γ → program α γ
-
-export Sequential (andThen)
-
-infixl:50 " >=> " => andThen
+--
+-- Creational
+--
 
 def let_
     [Functional program]
@@ -75,23 +122,37 @@ def let_
 
 def in_ : α → α := id
 
-class Conditional
-    (program : Type → Type → Type) where
-  sum {α β γ : Type} :
-    program γ α → program β α → program (γ ⊕ β) α
+def onlyFirst
+    [Functional program]
+    [Creational program]
+    [Sequential program] :
+  program α β → program (α × γ) (β × γ) :=
+    λ αpβ => (first >=> αpβ) &&& second
 
-export Conditional (sum)
+infixl:50 " <&& " => onlyFirst
 
-infixl:55 " ||| " => sum
+def onlySecond
+    [Functional program]
+    [Creational program]
+    [Sequential program] :
+  program β γ → program (α × β) (α × γ) :=
+    λ βpγ => first &&& (second >=> βpγ)
 
-def trueToLeftFalseToRightF : α × Bool → α ⊕ α
-  | ⟨α, true⟩ => .inl α
-  | ⟨α, false⟩ => .inr α
+infixl:50 " &&> " => onlySecond
 
-def trueToLeftFalseToRight
-    [Functional program] :
-  program (α × Bool) (α ⊕ α) :=
-    asProgram trueToLeftFalseToRightF
+def both
+      [Functional program]
+      [Sequential program]
+      [Creational program] :
+    program α γ → program β δ → program (α × β) (γ × δ) :=
+      λ αpγ βpδ =>
+        onlyFirst αpγ >=> onlySecond βpδ
+
+infixl:50 " <&> " => both
+
+--
+-- Conditional
+--
 
 def if_
     [Functional program]
@@ -105,8 +166,11 @@ def if_
     λ αpb t_apβ f_apβ =>
       let_ αpb $
         in_ $
-          trueToLeftFalseToRight >=>
+          asProgram (
+            λ αab => match αab with
+              | ⟨α, true⟩ => .inl α
+              | ⟨α, false⟩ => .inr α
+          ) >=>
           t_apβ ||| f_apβ
 
 def else_ : α → α := id
-
