PSBP/Laws/ProgramLaws.lean
@@ -1,0 +1,91 @@
+import PSBP.Specifications.ProgramSpecifications
+
+class LawfulFunctional (program : Type → Type → Type)
+    [Functional program]
+    [Sequential program] : Prop where
+  functional_identity :
+    (asProgram id : program α α) =
+      identity
+  functional_sequential
+      (αfβ : α → β)
+      (βfγ : β → γ) :
+    (asProgram αfβ >=> asProgram βfγ : program α γ) =
+      asProgram (βfγ ∘ αfβ)
+
+class LawfulFunctorial (program : Type → Type → Type)
+    [Functorial program] : Prop where
+  functorial_identity
+      (αpβ : program α β) :
+    (αpβ >-> id : program α β) =
+      αpβ
+  functorial_sequential
+      (αpβ : program α β)
+      (βfγ : β → γ)
+      (γfδ : γ → δ) :
+    (αpβ >-> βfγ >-> γfδ) =
+      (αpβ >-> (γfδ ∘ βfγ))
+
+class LawfulSequential (program : Type → Type → Type)
+    [Functional program]
+    [Sequential program] : Prop where
+  sequential_right_identity
+      (αpβ : program α β) :
+    (αpβ >=> identity : program α β) =
+      αpβ
+  sequential_left_identity
+      (αpβ : program α β) :
+    (identity >=> αpβ : program α β) =
+      αpβ
+  sequential_associativity
+      (αpβ : program α β)
+      (βpγ : program β γ)
+      (γpδ : program γ δ) :
+    ((αpβ >=> βpγ) >=> γpδ) =
+      (αpβ >=> (βpγ >=> γpδ))
+
+class LawfulCreational (program : Type → Type → Type)
+    [Functional program]
+    [Sequential program]
+    [Creational program] : Prop where
+  creational_onlyFirst_asProgram
+      (αfβ : α → β) :
+    (onlyFirst (asProgram αfβ)
+      : program (α × γ) (β × γ)) =
+      applyAtFirst αfβ
+  creational_onlyFirst_sequential
+      (αpβ : program α β)
+      (βpγ : program β γ) :
+    (onlyFirst (αpβ >=> βpγ) :
+      program (α × δ) (γ × δ)) =
+      (onlyFirst αpβ >=> onlyFirst βpγ)
+  creational_onlyFirst_first
+      (αpβ : program α β) :
+    (onlyFirst αpβ >=> (first : program (β × γ) β)
+      : program (α × γ) β) =
+      ((first : program (α × γ) α) >=> αpβ)
+  creational_onlyFirst_applyAtSecond
+      (αpβ : program α β)
+      (γfδ : γ → δ) :
+    (onlyFirst αpβ >=> applyAtSecond γfδ
+      : program (α × γ) (β × δ)) =
+      (applyAtSecond γfδ >=> onlyFirst αpβ)
+  creational_onlyFirst_assoc
+      (αpβ : program α β) :
+    (onlyFirst (onlyFirst αpβ) >=> assoc
+      : program ((α × γ) × δ) (β × (γ × δ))) =
+      (assoc >=> onlyFirst αpβ)
+
+class LawfulConditional (program : Type → Type → Type)
+    [Functional program]
+    [Sequential program]
+    [Conditional program] : Prop where
+  conditional_left
+      (γpα : program γ α)
+      (βpα : program β α) :
+    (left >=> γpα ||| βpα) =
+      γpα
+  conditional_right
+      (γpα : program γ α)
+      (βpα : program β α) :
+    (right >=> γpα ||| βpα) =
+      βpα
