PSBP/Theorems/ProgramTheorems.lean
@@ -1,0 +1,354 @@
+import PSBP.Specifications.ProgramSpecifications
+
+import PSBP.Laws.ProgramLaws
+
+import PSBP.Structures.ComputationValuedFunction
+
+import PSBP.Implementations.ProgramImplementations
+
+set_option linter.unusedVariables false
+
+open Function
+
+@[simp] theorem functional_identity
+  {α : Type}
+    [Applicative computation] :
+    (identity : FromComputationValuedFunction computation α α)
+      = asProgram id := by
+  calc
+    identity
+        = asProgram id
+          := rfl
+
+theorem functional_sequential'
+  {α β γ : Type}
+    [Monad computation]
+    [LawfulMonad computation]
+  (αfβ : α → β)
+  (βfγ : β → γ) :
+    (asProgram αfβ >=> asProgram βfγ :
+      FromComputationValuedFunction computation α γ)
+      = asProgram (βfγ ∘ αfβ) := by
+  calc
+    (asProgram αfβ >=> asProgram βfγ :
+      FromComputationValuedFunction computation α γ)
+        = (⟨λ α => pure $ αfβ α⟩ >=> ⟨λ β => pure $ βfγ β⟩)
+          := rfl
+    _   = ⟨λ α => (pure $ αfβ α) >>= λ β => pure $ βfγ β⟩
+          := rfl
+    _   = ⟨λ α => pure $ βfγ (αfβ α)⟩
+          := congrArg
+               FromComputationValuedFunction.mk
+               (funext λ α => pure_bind (αfβ α) (λ β => pure $ βfγ β))
+    _   = ⟨λ α => pure $ (βfγ ∘ αfβ) α⟩
+          := rfl
+    _   = asProgram (βfγ ∘ αfβ)
+          := rfl
+
+@[simp] theorem functional_sequential
+  {α β γ : Type}
+    [Monad computation]
+    [LawfulMonad computation]
+  (αfβ : α → β)
+  (βfγ : β → γ) :
+    (asProgram αfβ >=> asProgram βfγ :
+      FromComputationValuedFunction computation α γ)
+      = asProgram (βfγ ∘ αfβ) := by
+    simp[asProgram, andThen]
+
+theorem functorial_identity'
+  {α β : Type}
+    [Functor computation]
+    [LawfulFunctor computation]
+  (αpβ : FromComputationValuedFunction computation α β) :
+    (αpβ >-> id :
+      FromComputationValuedFunction computation α β)
+      = αpβ := by
+  let αfcβ := αpβ.toComputationValuedFunction
+  calc
+    (αpβ >-> id)
+        = ⟨λ α => id <$> αfcβ α⟩
+          := rfl
+    _   = ⟨λ α => αfcβ α ⟩
+          := congrArg
+               FromComputationValuedFunction.mk
+               (funext λ α => id_map (αfcβ α))
+    _   = ⟨αfcβ⟩
+          := rfl
+
+@[simp] theorem functorial_identity
+  {α β : Type}
+    [Functor computation]
+    [LawfulFunctor computation]
+  (αpβ : FromComputationValuedFunction computation α β) :
+    (αpβ >-> id :
+      FromComputationValuedFunction computation α β)
+      = αpβ := by
+    simp[andThenF]
+
+theorem functorial_sequential'
+  {α β γ δ : Type}
+    [Functor computation]
+    [LawfulFunctor computation]
+  (αpβ : FromComputationValuedFunction computation α β)
+  (βfγ : β → γ)
+  (γfδ : γ → δ) :
+    ((αpβ >-> βfγ) >-> γfδ :
+      FromComputationValuedFunction computation α δ)
+      = (αpβ >-> (γfδ ∘ βfγ)) := by
+  let αfcβ := αpβ.toComputationValuedFunction
+  calc
+    ((αpβ >-> βfγ) >-> γfδ)
+        = (⟨λ α => βfγ <$> αfcβ α⟩ >-> γfδ)
+          := rfl
+    _   = ⟨λ α => γfδ <$> (λ α => βfγ <$> αfcβ α) α⟩
+          := rfl
+    _   = ⟨λ α => γfδ <$> βfγ <$> αfcβ α⟩
+          := rfl
+    _   = ⟨λ α => (γfδ ∘ βfγ) <$> αfcβ α⟩
+          := congrArg
+               FromComputationValuedFunction.mk
+               (funext λ α => Eq.symm (comp_map βfγ γfδ (αfcβ α)))
+    _   = (αpβ >-> (γfδ ∘ βfγ))
+          := rfl
+
+@[simp] theorem functorial_sequential
+    {α β γ δ : Type}
+    [Functor computation]
+    [LawfulFunctor computation]
+  (αpβ : FromComputationValuedFunction computation α β)
+  (βfγ : β → γ)
+  (γfδ : γ → δ) :
+    ((αpβ >-> βfγ) >-> γfδ :
+      FromComputationValuedFunction computation α δ)
+      = (αpβ >-> (γfδ ∘ βfγ)) := by simp[andThenF, comp_map]
+
+
+theorem sequential_right_identity'
+  {α β : Type}
+    [Monad computation]
+    [LawfulMonad computation]
+  (αpβ : FromComputationValuedFunction computation α β) :
+    (αpβ >=> asProgram id :
+      FromComputationValuedFunction computation α β)
+    = αpβ := by
+   let αfcβ := αpβ.toComputationValuedFunction
+   calc
+      (αpβ >=> asProgram id :
+          FromComputationValuedFunction computation α β)
+          = ⟨λ α => αfcβ α >>= λ β => pure (id β)⟩
+            := rfl
+      _   = ⟨λ α => id <$> αfcβ α⟩
+            := congrArg
+                 FromComputationValuedFunction.mk
+                 (funext λ α => bind_pure_comp id (αfcβ α))
+      _   = ⟨λ α => αfcβ α⟩
+            := congrArg
+                 FromComputationValuedFunction.mk
+                 (funext λ α => id_map (αfcβ α))
+      _   = αpβ
+            := rfl
+
+@[simp] theorem sequential_right_identity
+  {α β : Type}
+    [Monad computation]
+    [LawfulMonad computation]
+  (αpβ : FromComputationValuedFunction computation α β) :
+    ((αpβ >=> asProgram id) :
+      FromComputationValuedFunction computation α β)
+      = αpβ := by simp[andThen]
+
+theorem sequential_left_identity'
+  {α β : Type}
+    [Monad computation]
+    [LawfulMonad computation]
+  (αpβ : FromComputationValuedFunction computation α β) :
+    (asProgram id >=> αpβ :
+      FromComputationValuedFunction computation α β)
+    = αpβ := by
+    let αfcβ := αpβ.toComputationValuedFunction
+    calc
+      (asProgram id >=> ⟨αfcβ⟩ :
+        FromComputationValuedFunction computation α β)
+          = ⟨λ α => pure α >>= αfcβ⟩
+            := rfl
+      _   = ⟨λ α => αfcβ α⟩
+            := congrArg
+                 FromComputationValuedFunction.mk
+                 (funext λ α => pure_bind α αfcβ)
+      _   = ⟨αfcβ⟩
+            := rfl
+
+@[simp] theorem sequential_left_identity
+  {α β : Type}
+    [Monad computation]
+    [LawfulMonad computation]
+  (αpβ : FromComputationValuedFunction computation α β) :
+    (asProgram id >=> αpβ :
+      FromComputationValuedFunction computation α β)
+    = αpβ := by simp[andThen]
+
+theorem sequential_associative'
+  {α β γ δ : Type}
+    [Monad computation]
+    [LawfulMonad computation]
+  (αpβ : FromComputationValuedFunction computation α β)
+  (βpγ : FromComputationValuedFunction computation β γ)
+  (γpδ : FromComputationValuedFunction computation γ δ) :
+    ((αpβ >=> βpγ) >=> γpδ :
+      FromComputationValuedFunction computation α δ) =
+      (αpβ >=> (βpγ >=> γpδ)) := by
+  let αfcβ : α → computation β := αpβ.toComputationValuedFunction
+  let βfcγ : β → computation γ := βpγ.toComputationValuedFunction
+  let γfcδ : γ → computation δ := γpδ.toComputationValuedFunction
+  let βfcδ : β → computation δ := λ β => βfcγ β >>= γfcδ
+  calc
+    ((αpβ >=> βpγ) >=> γpδ :
+      FromComputationValuedFunction computation α δ)
+        = (⟨λ α => αfcβ α >>= βfcγ⟩ >=> ⟨γfcδ⟩)
+          := rfl
+    _   = ⟨λ α => αfcβ α >>= βfcγ >>= γfcδ⟩
+          := rfl
+    _   = ⟨λ α => αfcβ α >>= (λ β => βfcγ β >>= γfcδ)⟩
+          := congrArg
+               FromComputationValuedFunction.mk
+               (funext λ α => bind_assoc (αfcβ α) βfcγ γfcδ)
+    _   = (⟨λ α => αfcβ α >>= βfcδ⟩ :
+            FromComputationValuedFunction computation α δ)
+          := rfl
+    _   = (αpβ >=> (βpγ >=> γpδ):
+            FromComputationValuedFunction computation α δ)
+          := rfl
+
+@[simp] theorem sequential_associative
+  {α β γ δ : Type}
+    [Monad computation]
+    [LawfulMonad computation]
+  (αpβ : FromComputationValuedFunction computation α β)
+  (βpγ : FromComputationValuedFunction computation β γ)
+  (γpδ : FromComputationValuedFunction computation γ δ) :
+    ((αpβ >=> βpγ) >=> γpδ :
+      FromComputationValuedFunction computation α δ) =
+      (αpβ >=> (βpγ >=> γpδ)) := by simp[andThen]
+
+theorem creational_onlyFirst_asProgram'
+  {α β γ : Type}
+    [Monad computation]
+    [LawfulMonad computation]
+  (αfβ : α → β) :
+    (onlyFirst (asProgram αfβ) :
+      FromComputationValuedFunction computation (α × γ) (β × γ)) =
+      (asProgram (λ (α, γ) => (αfβ α, γ))) := by
+  calc
+    (onlyFirst (asProgram αfβ))
+        = onlyFirst ⟨λ α => pure $ αfβ α⟩ :=
+        rfl
+    _   = ((first : FromComputationValuedFunction computation (α × γ) α) >=>
+            (⟨λ α => pure $ αfβ α⟩)) &&& second :=
+        rfl
+    _   = (((asProgram λ (α, _) => α) :
+            FromComputationValuedFunction computation (α × γ) α) >=>
+              (⟨λ α => pure $ αfβ α⟩)) &&& second :=
+        rfl
+    _   = ((⟨λ (α, _) => pure α⟩ :
+            FromComputationValuedFunction computation (α × γ) α) >=>
+              (⟨λ α => pure $ αfβ α⟩)) &&& second :=
+        rfl
+    _   = (⟨λ (α, _) => pure α >>= (λ α => pure $ αfβ α)⟩ :
+            FromComputationValuedFunction computation (α × γ) β) &&& second :=
+        rfl
+    _   = (⟨(λ (α, _) => pure $ αfβ α)⟩ :
+            FromComputationValuedFunction computation (α × γ) β) &&& second :=
+        congrArg
+          (λ (αfcβ : α → computation β) => ((⟨λ (α, _) => αfcβ α⟩ :
+            FromComputationValuedFunction computation (α × γ) β) &&& second))
+          (funext (λ α => pure_bind α (λ α => pure $ αfβ α)))
+    _   = (⟨λ (α, _) => pure $ αfβ α⟩ :
+            FromComputationValuedFunction computation (α × γ) β) &&& second :=
+        rfl
+    _   = (⟨λ (α, _) => pure $ αfβ α⟩ :
+            FromComputationValuedFunction computation (α × γ) β) &&&
+              (asProgram (λ (_, γ) => γ) :
+                FromComputationValuedFunction computation (α × γ) γ) :=
+        rfl
+    _   = (⟨λ (α, _) => pure $ αfβ α⟩ :
+            FromComputationValuedFunction computation (α × γ) β) &&&
+              (⟨λ (_, γ) => pure $ γ⟩ :
+                FromComputationValuedFunction computation (α × γ) γ) :=
+        rfl
+    _   = (⟨λ (α, γ) => (Prod.mk <$> (pure $ αfβ α)) <*> (pure $ γ)⟩ :
+             FromComputationValuedFunction computation (α × γ) (β × γ)) :=
+        rfl
+    _   = (⟨λ (α, γ) => (pure $ Prod.mk (αfβ α)) <*> (pure $ γ)⟩ :
+             FromComputationValuedFunction computation (α × γ) (β × γ)) :=
+        congrArg
+         (FromComputationValuedFunction.mk ∘
+           ((λ αfβaγ => λ (α, γ) => αfβaγ α <*> (pure $ γ)) :
+             (α → computation (γ → (β × γ))) → ((α × γ) → computation (β × γ))))
+          (funext λ α => (map_pure (Prod.mk) (αfβ α)))
+    _   = (⟨λ (α, γ) => Prod.mk (αfβ α) <$> (pure $ γ)⟩) :=
+        congrArg
+         FromComputationValuedFunction.mk
+          (funext λ (α, γ) => (pure_seq (Prod.mk (αfβ α)) (pure $ γ)))
+    _   = (⟨λ (α, γ) => pure (Prod.mk (αfβ α) γ)⟩) :=
+        congrArg
+         FromComputationValuedFunction.mk
+          (funext λ (α, γ) => (map_pure (Prod.mk (αfβ α)) γ))
+    _   = (⟨λ (α, γ) => pure $ (αfβ α, γ)⟩) :=
+        rfl
+    _   = (asProgram (λ (α, γ) => (αfβ α, γ))) :=
+        rfl
+
+@[simp] theorem creational_onlyFirst_asProgram
+  {α β γ : Type}
+    [Monad computation]
+    [LawfulMonad computation]
+  (αfβ : α → β) :
+    (onlyFirst (asProgram αfβ) :
+      FromComputationValuedFunction computation (α × γ) (β × γ)) =
+      (asProgram (λ (α, γ) => (αfβ α, γ)))
+      := by simp [onlyFirst, asProgram, product, first, second]
+
+@[simp] theorem creational_onlyFirst_sequential
+  {α β γ : Type}
+    [Monad computation]
+    [LawfulMonad computation]
+  (αpβ : FromComputationValuedFunction computation α β)
+  (βpγ : FromComputationValuedFunction computation β γ) :
+    (onlyFirst (αpβ >=> βpγ) :
+      FromComputationValuedFunction computation (α × δ) (γ × δ)) =
+      (onlyFirst αpβ >=> onlyFirst βpγ :
+        FromComputationValuedFunction
+          computation (α × δ) (γ × δ)) := by
+          simp[onlyFirst, andThen, asProgram, product, first, second]
+
+@[simp] theorem creational_onlyFirst_first
+  {α β γ : Type}
+    [Monad computation]
+    [LawfulMonad computation]
+  (αpβ : FromComputationValuedFunction computation α β) :
+    (onlyFirst αpβ >=> (first : FromComputationValuedFunction computation (β × γ) β)
+      : FromComputationValuedFunction computation (α × γ) β) =
+      ((first : FromComputationValuedFunction computation (α × γ) α) >=> αpβ) := by
+          simp[onlyFirst, andThen, asProgram, product, first, second]
+
+@[simp] theorem creational_onlyFirst_applyAtSecond
+  {α β γ δ : Type}
+    [Monad computation]
+    [LawfulMonad computation]
+  (αpβ : FromComputationValuedFunction computation α β)
+  (γfδ : γ → δ) :
+    (onlyFirst αpβ >=> applyAtSecond γfδ
+      : FromComputationValuedFunction computation (α × γ) (β × δ)) =
+      (applyAtSecond γfδ >=> onlyFirst αpβ) := by
+          simp[onlyFirst, andThen, applyAtSecond, asProgram, product, first, second]
+
+@[simp] theorem creational_onlyFirst_assoc
+  {α β γ δ : Type}
+    [Monad computation]
+    [LawfulMonad computation]
+  (αpβ : FromComputationValuedFunction computation α β) :
+    (onlyFirst (onlyFirst αpβ) >=> assoc
+      : FromComputationValuedFunction computation ((α × γ) × δ) (β × (γ × δ))) =
+      (assoc >=> onlyFirst αpβ) := by
+          simp[onlyFirst, andThen, asProgram, product, first, second, assoc]
